Ajout suite exemple chapitre 3

examples/parser.v
@@ -13,10 +13,10 @@ Definition data := list octet.
 Definition Decodeur X := data -> option (X * data).
 
 Definition decode {X} (d : Decodeur X) (l : data) : option X :=
- match d l with
- | None => None
- | Some (v, _) => Some v
- end.
+  match d l with
+  | None => None
+  | Some (v, _) => Some v
+  end.
 
 Definition decode_pair : Decodeur (octet * octet) :=
   fun d =>
@@ -27,12 +27,12 @@ Definition decode_pair : Decodeur (octet * octet) :=
 
 Definition fmap {X Y} (f : X -> Y) (e : Decodeur X) : Decodeur Y :=
   fun d => match e d with
-        | None => None
-        | Some (v, s) => Some (f v, s)
-        end.
+           | None => None
+           | Some (v, s) => Some (f v, s)
+           end.
 
 Definition decode_add : Decodeur N :=
- fmap (fun v => fst v + snd v) decode_pair.
+  fmap (fun v => fst v + snd v) decode_pair.
 
 Definition decode_mult : Decodeur N :=
   fmap (fun v => fst v * snd v) decode_pair.
@@ -42,9 +42,9 @@ Reset decode_pair.
 
 Definition fmap {X Y} (f : X -> Y) (e : Decodeur X) : Decodeur Y :=
   fun d => match e d with
-        | None => None
-        | Some (v, s) => Some (f v, s)
-        end.
+           | None => None
+           | Some (v, s) => Some (f v, s)
+           end.
 
 
 Lemma fmap_id : forall X (d : Decodeur X), fmap id d = d.
@@ -63,9 +63,9 @@ Qed.
 
 Definition app {X Y} (f : Decodeur (X -> Y)) (x : Decodeur X) : Decodeur Y :=
   fun s => match f s with
-        | None => None
-        | Some (f,s) => fmap f x s
-        end.
+           | None => None
+           | Some (f,s) => fmap f x s
+           end.
 
 Notation " f '<*>' g" := (app f g)(at level 50).
 
@@ -107,9 +107,9 @@ Definition decode_pair : Decodeur (octet * octet) :=
 
 Definition bind {X Y} (d : Decodeur X) (f : X -> Decodeur Y) : Decodeur Y :=
   fun s => match d s with
-        | None => None
-        | Some (v,s) => f v s
-        end.
+           | None => None
+           | Some (v,s) => f v s
+           end.
 
 Notation "'let!' v ':=' f 'in' g" := (bind f (fun v => g))(at level 50).
 Notation "'ret!' v" := (pure v)(at level 50).
@@ -134,7 +134,7 @@ Proof.
 Qed.
 
 Definition to_u32 (a0 a1 a2 a3 : octet) : N :=
- a0 * (N.pow 2 32) + a1 * (N.pow 2 16) + a2  * (N.pow 2 8) + a3.
+  a0 * (N.pow 2 32) + a1 * (N.pow 2 16) + a2  * (N.pow 2 8) + a3.
 
 Definition decode_packet_length : Decodeur N :=
   pure to_u32 <*> decode_next <*> decode_next <*> decode_next <*> decode_next.
@@ -155,11 +155,11 @@ Next Obligation.
 Defined.
 
 Equations take (n : N) : Decodeur data by wf (N.to_nat n) Nat.lt :=
- take 0 := ret! [];
- take n :=
-   let! v := decode_next in
-   let! vs := take (pred n) in
-   ret! (v :: vs).
+  take 0 := ret! [];
+  take n :=
+    let! v := decode_next in
+    let! vs := take (pred n) in
+    ret! (v :: vs).
 Next Obligation.
 Abort.
 
@@ -183,47 +183,51 @@ Compute (decode decode_payload_SSH test).
 Reset Decodeur.
 
 From Formalisation Require Export Span.
+From FreeMonad Require Import FreeMonad.
+From SepLogic Require Import SepSet.
+From Formalisation Require Import IsFresh Inject.
 
-Definition Decodeur (X : Type) := data -> span -> option (X * span).
+
+Definition DecodeurM (X : Type) := data -> span -> option (X * span).
 
 Equations length (l: data) : N :=
   length nil := 0;
   length (_ :: t) := N.succ (length t).
 
-Definition decode {X} (d : Decodeur X) (l : data) : option X :=
+Definition decodeM {X} (d : DecodeurM X) (l : data) : option X :=
   match d l (mk_span 0 (length l)) with
   | None => None
   | Some (v, _) => Some v
   end.
 
-Definition pure {X} (v : X) : Decodeur X := fun data l => Some (v,l).
+Definition pure {X} (v : X) : DecodeurM X := fun data l => Some (v,l).
 
-Definition bind {X Y} (d : Decodeur X) (k : X -> Decodeur Y) : Decodeur Y :=
- fun data l =>
-  match d data l with
-  | None => None
-  | Some (v, s) => k v data s
-  end.
+Definition bind {X Y} (d : DecodeurM X) (k : X -> DecodeurM Y) : DecodeurM Y :=
+  fun data l =>
+    match d data l with
+    | None => None
+    | Some (v, s) => k v data s
+    end.
 
-Notation "'let!' v ':=' f 'in' g" := (bind f (fun v => g))(at level 50).
-Notation "'ret!' v" := (pure v)(at level 50).
+Notation "'let!' v ':=' f 'in' g" := (bind f (fun v => g)) (v name, at level 50).
+Notation "'ret!' v" := (pure v) (at level 50).
 
-Definition app {X Y} (a : Decodeur (X -> Y)) (d : Decodeur X) : Decodeur Y :=
+Definition app {X Y} (a : DecodeurM (X -> Y)) (d : DecodeurM X) : DecodeurM Y :=
   let! f := a in
   let! x := d in
   ret! (f x).
 
 Notation " f '<*>' g" := (app f g)(at level 50).
 
-Definition take (n : N) : Decodeur span :=
+Definition takeM (n : N) : DecodeurM span :=
   fun _ s =>
-   if n <=? len s
-   then
-    let res := mk_span (pos s) n in
-    let sres := mk_span (pos s + n) (len s - n) in
-    Some (res, sres)
-   else
-    None.
+    if n <=? len s
+    then
+      let res := mk_span (pos s) n in
+      let sres := mk_span (pos s + n) (len s - n) in
+      Some (res, sres)
+    else
+      None.
 
 Equations lookup (n : N) (l : data) : option N by wf (N.to_nat n) Nat.lt :=
   lookup n [] := None;
@@ -233,7 +237,7 @@ Next Obligation.
   lia.
 Defined.
 
-Definition read (s : span) (n : N) : Decodeur N :=
+Definition readM (s : span) (n : N) : DecodeurM N :=
   fun d t =>
     if n <? len s
     then
@@ -244,27 +248,322 @@ Definition read (s : span) (n : N) : Decodeur N :=
     else
       None.
 
-Definition decode_first : Decodeur N :=
-  let! s := take 1 in
-  read s 0.
+Definition decode_nextM : DecodeurM N :=
+  let! s := takeM 1 in
+  readM s 0.
 
-Definition fail {X} : Decodeur X := fun _ _ => None.
+Definition failM {X} : DecodeurM X := fun _ _ => None.
 
 Definition to_u32 (a0 a1 a2 a3 : octet) : N :=
- a0 * (N.pow 2 32) + a1 * (N.pow 2 16) + a2  * (N.pow 2 8) + a3.
+  a0 * (N.pow 2 32) + a1 * (N.pow 2 16) + a2  * (N.pow 2 8) + a3.
 
-Definition decode_packet_length : Decodeur N :=
-  pure to_u32 <*> decode_first <*> decode_first <*> decode_first <*> decode_first.
+Definition decode_packet_length : DecodeurM N :=
+  pure to_u32 <*> decode_nextM <*> decode_nextM <*> decode_nextM <*> decode_nextM.
 
-Definition decode_payload_SSH : Decodeur span :=
+Definition decode_payload_SSH : DecodeurM span :=
   let! packet_length := decode_packet_length in
-  let! padding_length := decode_first in
-  let! payload := take (packet_length - padding_length - 1) in
-  let! padding := take padding_length in
+  let! padding_length := decode_nextM in
+  let! payload := takeM (packet_length - padding_length - 1) in
+  let! padding := takeM padding_length in
   ret! payload.
 
 Definition test := [0;0;0;5;1;0;1;2;15].
 
-Compute (decode decode_payload_SSH test).
+Compute (decodeM decode_payload_SSH test).
 
-Reset Decodeur.
+
+Inductive DECODE : Type -> Type :=
+| TakeOp : N -> DECODE span
+| ReadOp : span -> N -> DECODE octet
+| FailOp : forall {X}, DECODE X.
+
+Definition Decodeur := Free DECODE.
+
+Definition take (n : N) : Decodeur span := syntax_effect (TakeOp n).
+
+Definition read (s : span) (pos : N): Decodeur N := syntax_effect (ReadOp s pos).
+
+Definition fail {X} : Decodeur X := syntax_effect FailOp.
+
+Fixpoint wp {X} (m: Decodeur X) (Q : X -> iProp) : iProp :=
+  match m with
+  | ret v => Q v
+  | op (TakeOp n) k => ∀ v, IsFresh v -∗ wp (k v) Q
+  | op (ReadOp s n) k => ∀ v , wp (k v) Q
+  | op FailOp _ => True
+  end.
+
+Local Open Scope free_monad_scope.
+
+Lemma wp_bind {X Y} (e : Decodeur X) (f :  X → Decodeur Y) (Q : Y -> iProp) (Q' : X -> iProp) :
+  wp e Q' ⊢
+    (∀ v,  Q' v -∗ wp (f v) Q ) -∗
+    wp (let! v := e in f v) Q %I.
+Proof.
+  iIntros "HA HB". revert e. fix e 1.
+  destruct e0 as [v | Z []]; simpl; auto.
+  - iApply ("HB" with "HA").
+  - iIntros (v) "HC". iDestruct ("HA" with "HC") as "HA".
+    iPoseProof "HB" as "HB". apply e.
+  - iIntros (v). iDestruct ("HA" $! v) as "HA".
+    iPoseProof "HB" as "HB". apply e.
+Qed.
+
+Lemma wp_consequence {X} (P Q : X -> iProp) (f : Decodeur X) :
+  ⊢ wp f P -∗
+    (∀ x, P x -∗ Q x) -∗
+    wp f Q.
+Proof.
+  induction f as [v | Y [] k]; simpl; intros; auto.
+  - iIntros "HA HB". iApply ("HB" with "HA").
+  - iIntros "HA HB * HC". iDestruct ("HA" with "HC") as "HA".
+    iApply (H with "HA HB").
+  - iIntros "HA HB" (v). iApply (H with "HA HB").
+Qed.
+
+
+Notation "{{ P }} m {{ v ; Q }}" := (P ⊢ wp m (fun v => Q))
+                                      (at level 20,
+                                        format "'[hv' {{  P  }}  '/  ' m  '/'  {{  v ;  Q  }} ']'").
+
+Lemma rule_ret {X} (v : X) H (Q : X -> iProp) :
+  (H ⊢ Q v) -> {{ H }} (ret v : Decodeur X) {{ v'; Q v' }}.
+Proof. simpl; iIntros. iApply H0; auto. Qed.
+
+Lemma rule_bind {X Y} (e : Decodeur X) (f : X -> Decodeur Y) Q Q' (H : iProp) :
+  ({{ H }} e {{ v; Q' v }}) ->
+  (∀ v, {{ Q' v }} f v {{ v'; Q v' }}) ->
+  {{ H }} do v <- e; f v {{ v; Q v}}.
+Proof.
+  intros. iIntros "HA".
+  iApply (wp_bind e f _ Q' with "[HA]").
+  - iApply (H0 with "[HA]"); auto.
+  - iIntros (v) "HC". iApply (H1 with "[HC]"); auto.
+Qed.
+
+Section Rules.
+
+  Variable X: Type.
+  Implicit Type P: iProp.
+  Implicit Type Q: X -> iProp.
+
+  Lemma rule_consequence: forall P P' Q Q' m,
+
+      ({{ P' }} m {{ v; Q' v }}) ->
+      (P ⊢ P') ->
+      (forall v, Q' v ⊢ Q v) ->
+      (*-----------------------*)
+      {{ P }} m {{ v; Q v }}.
+  Proof.
+    intros. iIntros "HA". iDestruct (H0 with "HA") as "HA".
+    iDestruct (H with "HA") as "HA". iApply (wp_consequence with "HA").
+    iIntros "*". iApply H1.
+  Qed.
+
+
+  Lemma frame_bind : forall (P : iProp), ⊢ P -∗ emp ∗ P.
+  Proof. iIntros "* $". Qed.
+
+  Lemma rule_frame: forall P Q P' m,
+
+      ({{ P }} m {{ v; Q v }}) ->
+      (*----------------------------*)
+      {{ P ∗ P' }} m {{ v; Q v ∗ P' }}.
+  Proof.
+    intros. iIntros "[HA HC]". iApply (wp_consequence with "[HA]").
+    iApply H; auto. iIntros; iFrame.
+  Qed.
+
+  Lemma rule_fail H Q : {{ H }} fail {{ v; Q v }}.
+  Proof. auto. Qed.
+
+  Lemma rule_read s res : {{ emp }} read s res {{ _; emp }}.
+  Proof. eauto. Qed.
+
+  Lemma rule_take n : {{ emp }} take n {{ v; IsFresh v }}.
+  Proof. simpl. eauto. Qed.
+
+End Rules.
+
+Record packet_SSHS (S : Type) :=
+  mk_ssh {
+      packet_length : N;
+      padding_length : N;
+      payload : S;
+      mac : S; }.
+
+Arguments mk_ssh [S].
+Arguments packet_length [S].
+Arguments padding_length [S].
+Arguments payload [S].
+Arguments mac [S].
+
+Definition packet_SSH := packet_SSHS span.
+
+Definition fold_r {A B} (f : A -> B -> B) (b : B) (p : packet_SSHS A) : B :=
+  f (payload p) (f (mac p) b).
+
+Definition decode_next : Decodeur N :=
+  let! s := take 1 in
+  read s 0.
+
+Lemma rule_next : {{ emp }} decode_next {{ _; True }}.
+Proof.
+  eapply rule_bind.
+  eapply rule_take.
+  intro. eapply rule_consequence. eapply rule_frame. eapply rule_read.
+  iIntros "HA". iSplitR; eauto. iApply "HA".
+  eauto.
+Qed.
+
+Definition decode_u32 :=
+  let! a := decode_next in
+  let! b := decode_next in
+  let! c := decode_next in
+  let! d := decode_next in
+  ret (to_u32 a b c d).
+
+Lemma rule_u32 : {{ emp }} decode_u32 {{ _; True }}.
+Proof.
+  eapply rule_bind.
+  eapply rule_next.
+  intro. eapply rule_bind.
+  eapply rule_consequence. eapply rule_frame. eapply rule_next.
+  iIntros "HA". iSplitR; eauto. iApply "HA". eauto.
+  intro. eapply rule_bind.
+  eapply rule_consequence. eapply rule_frame. eapply rule_next.
+  iIntros "HA". iSplitR; eauto. iApply "HA". eauto.
+  intro. eapply rule_bind.
+  eapply rule_consequence. eapply rule_frame. eapply rule_next.
+  iIntros "HA". iSplitR; eauto. iApply "HA". eauto.
+  eauto.
+Qed.
+
+Definition decode_packet_SSH : Decodeur packet_SSH :=
+  let! packet_length := decode_u32 in
+  let! padding_length := decode_next in
+  if padding_length + 1 <=? packet_length
+  then
+    let! payload := take (packet_length - padding_length - 1) in
+    let! padding := take padding_length in
+    let! mac := take 20 in
+    ret (mk_ssh packet_length padding_length payload mac)
+  else
+    fail.
+
+Close Scope free_monad_scope.
+
+Fixpoint eval {X} (m : Decodeur X) : DecodeurM X :=
+  match m with
+  | ret v => ret! v
+  | op (TakeOp n) k =>
+      let! v := takeM n in
+      eval (k v)
+  | op (ReadOp s pos) k =>
+      let! v := readM s pos in
+      eval (k v)
+  | op FailOp _ => failM
+  end.
+
+Definition decode {X} (d : Decodeur X) (data : data) : option X :=
+  match eval d data (mk_span 0 (length data)) with
+  | Some (v, _) => Some v
+  | _ => None
+  end.
+
+Lemma eval_monotone : forall X (e : Decodeur X) s1 s2 a v,
+    eval e a s1 = Some (v, s2) ->
+    (pos s1 <= pos s2)%N /\ (pos s2 + len s2 <= pos s1 + len s1)%N.
+Proof.
+  fix IH 2.
+  destruct e as [v  | Y []]; simpl; intros.
+  - inversion H. split; lia.
+  - unfold eval in H. fold (@eval X) in H. unfold bind in H. unfold takeM in H.
+    destruct ((n <=? len s1)%N) eqn:?. 2 : inversion H.
+    eapply IH in H as [P0 P1]. eapply N.leb_le in Heqb. simpl in *. lia.
+  - unfold eval in H. fold (@eval X) in H. unfold bind in H. unfold readM in H.
+    destruct ((n <? len s)%N) eqn:?. 2 : inversion H.
+    destruct (lookup (pos s + n) a). 2 : inversion H.
+    eapply IH in H as [P0 P1]. eapply N.ltb_lt in Heqb. lia.
+  - inversion H.
+Qed.
+
+Lemma soundness : forall X d H (Q : X -> iProp),
+    {{ H }} d {{v ; Q v }} ->
+    forall data s (v : X) s',
+      eval d data s = Some (v, s') ->
+      H ∗ injectSL (pos s) (pos s') ⊢ Q v.
+Proof.
+  fix IH 2.
+  destruct d as [v | Y []]; simpl; intros.
+  (* ret *)
+  - iIntros "[HA HB]". inversion H1. subst.
+    iDestruct (injectSL_emp with "HB") as "_". lia.
+    iApply (H0 with "HA").
+  (* take *)
+  - unfold eval in H1. fold (@eval X) in H1. unfold bind in H1. unfold takeM in H1.
+    destruct ((n <=? len s)%N) eqn:?.
+    2 : inversion H1.
+    epose H1 as grow.
+    eapply eval_monotone in grow as [P0 P1]. simpl in *.
+    iIntros "[HA HB]". iApply IH; eauto. simpl.
+    unfold injectSL. rewrite (inject_union (pos s + n)). 2-3 : lia.
+    iDestruct (big_sepS_union with "HB") as "[HC HB]". apply inject_disjoint.
+    iSplitR "HB"; eauto.
+    iApply (H0 with "HA [HC]").
+    iApply (inject_IsFresh with "HC"); simpl; lia.
+  (* read *)
+  - unfold eval in H1. fold (@eval X) in H1. unfold bind in H1. unfold readM in H1.
+    destruct ((n <? len s)%N) eqn:?. 2 : inversion H1.
+    destruct (lookup (pos s + n) data0). 2 : inversion H1.
+    iIntros "[HA HB]". iApply IH; eauto. iFrame. iApply (H0 with "HA").
+  (* fail *)
+  - inversion H1.
+Qed.
+
+Definition injectPos (start : N) (fin : N) : gset positive :=
+  set_map encode (inject start fin).
+
+Lemma encode_disj : forall (B : gset N) n,
+    n ∉ B -> ({[encode n]} : gset positive) ## set_map encode B.
+Proof.
+  induction B as [ | n0 set not_in IH] using set_ind_L; simpl; intros.
+  - rewrite set_map_empty. eapply disjoint_empty_r.
+  - repeat intro. apply elem_of_singleton_1 in H0. subst.
+    rewrite set_map_union_L in H1. apply elem_of_union in H1.
+    destruct H1.
+    + apply H. rewrite set_map_singleton_L in H0. apply elem_of_singleton in H0.
+      apply elem_of_union. left. apply elem_of_singleton. apply encode_inj. apply H0.
+    + assert (n ∉ set). intro. apply H. apply elem_of_union. right. apply H1.
+      apply IH in H1.
+      edestruct H1. eapply elem_of_singleton. reflexivity. eapply H0.
+Qed.
+
+
+Lemma lemma_final : forall start fin, && injectPos start fin ⊢ injectSL start fin.
+Proof.
+  iIntros (start fin).
+  unfold injectPos, injectSL.
+  induction (inject start fin) as [ | A B C D] using set_ind_L; iIntros "HA".
+  - rewrite set_map_empty. iApply big_sepS_empty. auto.
+  - rewrite set_map_union_L. iDestruct (heap_ctx_split with "HA") as "[HA HB]".
+    rewrite set_map_singleton. eapply encode_disj. eauto.
+    iApply big_sepS_union. apply disjoint_singleton_l. auto.
+    iSplitL "HA".
+    + rewrite set_map_singleton_L. iApply big_sepS_singleton. iFrame.
+    + iApply (D with "HB").
+Qed.
+
+
+Theorem adequacy : forall X d (Q : X -> Prop),
+    {{ emp }} d {{ v; ⌜Q v⌝ }} ->
+    forall data v,
+      decode d data = Some v ->
+      Q v.
+Proof.
+  intros. unfold decode in H0.
+  destruct (eval d data0) as  [[r s]| ] eqn:?. 2 : inversion H0.
+  injection H0. intro. subst. eapply soundness_pure.
+  iIntros "HA". iApply (soundness _ d emp (fun v => ⌜ Q v ⌝)); eauto.
+  iSplitR; auto. simpl. iApply lemma_final; eauto.
+Qed.
